Progress on bytestring

examples/bytestring/prims_verif.v
@@ -6,10 +6,100 @@ Require Import CertiGraph.CertiGC.spatial_gcgraph.
 Require Import VeriFFI.examples.bytestring.specs.
 
 Lemma representable_string_max_length:
+ (* NOT PROVABLE! *)
   forall (s: string) (g: graph) (p: rep_type),
    is_in_graph g s p ->
    graph_rep g |-- !! (Z.of_nat (String.length s) < Ptrofs.max_unsigned/4).
 Admitted.
+
+Lemma allocate_in_nursery_pf {n: Z} {nursery : space}
+   (H: 0 <= n <= nursery.(total_space)-nursery.(used_space)) :
+  0 <= nursery.(used_space)+n <= nursery.(total_space).
+Proof.
+intros.
+pose proof space_order nursery.
+lia.
+Qed.
+
+Definition allocate_in_nursery (n: Z) (nursery : space)
+   (H: 0 <= n <= nursery.(total_space)-nursery.(used_space)) :=
+  {| space_start := nursery.(space_start);
+     used_space := nursery.(used_space) + n;
+     total_space := nursery.(total_space);
+     space_sh := nursery.(space_sh);
+     space_order := allocate_in_nursery_pf H;
+     space_upper_bound := nursery.(space_upper_bound) |}.
+
+Lemma allocate_in_full_gc_aux:
+  forall n nursery H h,
+Zlength (allocate_in_nursery n nursery H :: tl (spaces h)) = MAX_SPACES.
+Proof.
+intros.
+pose proof spaces_size h.
+destruct (spaces h).
+inversion H0.
+simpl.
+rewrite Zlength_cons in *.
+auto.
+Qed.
+
+Print headroom.
+
+Lemma allocate_in_full_gc :
+ forall (n: Z) g t_info roots outlier ti sh gv
+  (H: 0 <= n <= headroom t_info),
+ full_gc g t_info roots outlier ti sh gv |--
+  let nursery := heap_head (ti_heap t_info) in
+  let t_info' := {| ti_heap_p := t_info.(ti_heap_p);
+                    ti_heap := {| spaces := allocate_in_nursery n nursery H ::
+                                      tl (spaces (ti_heap t_info));
+                                  spaces_size := allocate_in_full_gc_aux n nursery H _ |};
+                    ti_args := t_info.(ti_args);
+                    arg_size := t_info.(arg_size);
+                    ti_frames := t_info.(ti_frames);
+                    ti_nalloc := t_info.(ti_nalloc) |}
+ in @data_at_ env_graph_gc.CompSpecs sh (tarray int_or_ptr_type n)
+      (offset_val (WORD_SIZE * used_space (heap_head (ti_heap t_info'))) 
+       (space_start (heap_head (ti_heap t_info'))))
+   * full_gc g t_info' roots outlier ti sh gv.
+Proof.
+intros.
+unfold full_gc.
+Intros.
+destruct H0 as [? [? ? ] ].
+entailer!!.
+-
+ split3; auto; simpl.
+ + admit.
+ + destruct H1 as [? [ ? [? ?] ] ].
+   split3; [ | | split]; auto.
+   admit.
+-
+  simpl.
+  admit.
+Admitted.
+
+ Lemma get_tinfo_alloc:
+  forall g t_info roots outlier ti sh gv,
+  full_gc g t_info roots outlier ti sh gv |--
+  @field_at env_graph_gc.CompSpecs sh env_graph_gc.thread_info_type (DOT _alloc) 
+       (offset_val (WORD_SIZE * used_space (heap_head (ti_heap t_info)))
+             (space_start (heap_head (ti_heap t_info)))) ti
+    * (@field_at env_graph_gc.CompSpecs sh env_graph_gc.thread_info_type (DOT _alloc) 
+       (offset_val (WORD_SIZE * used_space (heap_head (ti_heap t_info)))
+             (space_start (heap_head (ti_heap t_info)))) ti -* 
+       full_gc g t_info roots outlier ti sh gv).
+Proof.
+ intros.
+ unfold full_gc.
+ Intros.
+ rewrite prop_true_andp by auto.
+ unfold before_gc_thread_info_rep.
+ unfold_data_at (data_at _ _ _ _).
+ cancel.
+ rewrite <- wand_sepcon_adjoint.
+ cancel.
+Qed.
 
 Lemma body_pack:
   semax_body Vprog Gprog f_pack pack_spec.
@@ -44,7 +134,7 @@ Proof.
             lvar ___FRAME__ (Tstruct _stack_frame noattr) v___FRAME__;
             lvar ___ROOT__ (tarray int_or_ptr_type 1) v___ROOT__; 
             gvars gv; temp _tinfo ti; temp _save0 (rep_type_val g p))
-     SEP (full_gc g t_info roots outlier ti sh gv;
+     SEP (full_gc g t_info roots outlier ti sh gv; library.mem_mgr gv;
           frame_rep_ Tsh v___FRAME__ v___ROOT__ (ti_fp t_info) 1))
    break: 
     (PROP ()
@@ -52,7 +142,7 @@ Proof.
             lvar ___FRAME__ (Tstruct _stack_frame noattr) v___FRAME__;
             lvar ___ROOT__ (tarray int_or_ptr_type 1) v___ROOT__; 
             gvars gv; temp _tinfo ti; temp _save0 (rep_type_val g p))
-     SEP (full_gc g t_info roots outlier ti sh gv;
+     SEP (full_gc g t_info roots outlier ti sh gv; library.mem_mgr gv;
           frame_rep_ Tsh v___FRAME__ v___ROOT__ (ti_fp t_info) 1)).
  - Exists x p. entailer!!. f_equal. f_equal. lia.
  - Intros s ps.
@@ -68,11 +158,26 @@ _get_Coq_Strings_String_string_tag (level 98).
    forward.
    forward.
    deadvars!.
-  set (len := Z.of_nat (String.length x)).
+  set (len := Z.of_nat (String.length x)) in *.
+  assert (LEN: 0 <= len < Int64.max_unsigned / 4) by rep_lia. clear H2.
   set (pad_length := 8 - len mod 8).
   set (n := (len + pad_length) / 8 + 1).
-  replace (Int64.add (Int64.divu _ _) _) with (Int64.repr n) by admit.
-   eapply semax_seq'.
+  replace (Int64.add (Int64.divu _ _) _) with (Int64.repr n).
+  2:{
+    change (Ptrofs.to_int64 _) with (Int64.repr 8).
+    unfold Int64.modu.
+    rewrite Int64.unsigned_repr
+       by (clear - LEN;  clearbody len; simpl in *; rep_lia).
+    rewrite Int64.unsigned_repr by rep_lia.
+     rewrite sub64_repr, add64_repr, divu_repr64, add64_repr.
+    f_equal; auto.
+    assert (0 <= len mod 8 < 8) by (apply Z.mod_bound_pos; lia).
+    clearbody len; clear - H2 LEN.
+    set (j := Int64.max_unsigned) in *; compute in j; subst j.
+    simpl in LEN. lia.
+    rep_lia.
+  }
+  eapply semax_seq'.
   +
    eapply semax_Delta_subsumption with GC_SAVE1_tycontext.
    apply prove_tycontext_sub; try reflexivity; repeat split; auto.
@@ -91,8 +196,113 @@ _get_Coq_Strings_String_string_tag (level 98).
   |  ]
  end.
 eapply semax_pre; [ | 
-  apply (semax_GC_SAVE1 n Espec gv sh ti outlier v___ROOT__ v___FRAME__ H); try eassumption].
+  apply (semax_GC_SAVE1 n Espec gv sh ti outlier v___ROOT__ v___FRAME__ H p _ x); try eassumption].
 entailer!!.
+* clear - LEN. clearbody len. subst n. subst pad_length.
+    assert (0 <= len < Int64.modulus / 4).
+    revert LEN.
+    really_simplify (Int64.modulus / 4).
+    really_simplify (Int64.max_unsigned / 4). intro. lia.
+    assert (0 <= (len + (8 - len mod 8)) / 8 + 1 < Int64.modulus/2).
+    2:{destruct H0; split; auto.
+       unfold Int64.max_signed, Int64.half_modulus. lia.
+    }
+    clear LEN.
+    change Int64.modulus with ((Int64.modulus/8)*8) in *.
+    change (Int64.modulus / 8 * 8 / 4) with (2*(Int64.modulus/8)) in H.
+    change (Int64.modulus/8*8/2) with (4*(Int64.modulus/8)).
+    assert (8 < Int64.modulus/8) by (simpl; lia).
+    set (N := Int64.modulus / 8) in *. clearbody N.
+    assert (0 <= len mod 8 < 8) by (apply Z.mod_bound_pos; lia).    
+    assert (0 <= (len + (8 - len mod 8)) / 8) by (apply Z_div_nonneg_nonneg; lia).
+    split; [lia | ].
+    assert (len + (8 - len mod 8) <= len + 8) by lia.
+    apply Z.le_lt_trans with ((len + 8)/8 + 1).
+    apply Z.add_le_mono_r.
+    apply Z.div_le_mono; try lia.
+    change 8 with (1*8) at 1; rewrite Z.div_add by lia.
+    clear - H H0.
+    apply Z.le_lt_trans with ((len+2) + (2*N-2)); try lia.
+    replace (len + 2 + (2*N-2)) with (len + (2*N-2) + 2) by lia.
+    rewrite <- Z.add_assoc. change (1+1) with 2.
+    apply Z.add_le_mono_r.
+    assert (len / 8 <= len) by (apply Z.div_le_upper_bound; lia).
+    lia.
+* eapply space_start_isptr'; eassumption.
+
++
+ Intros g' v0' roots' t_info'.
+ abbreviate_semax.
+ simpl app.
+
+ assert (0 < n). {
+   subst n.
+   assert (len mod 8 < 8) by (apply Z_mod_lt; lia).
+   assert (0 <= pad_length) by lia.  
+   assert (0 <= (len + pad_length) / 8) by (apply Z.div_pos; lia).
+   lia.
+  }
+
+ assert (H99: 0 <= n <=
+  total_space (heap_head (ti_heap t_info')) - used_space (heap_head (ti_heap t_info'))).
+ { clear - H2 H7. unfold headroom in H2. lia. }
+ sep_apply (allocate_in_full_gc n g' t_info' roots' outlier ti sh gv H99).
+ cbv zeta.
+ match goal with |- context [full_gc g' ?A] =>  set (t_info3 := A) end.
+ change (ti_fp t_info') with (ti_fp t_info3).
+ 
+ assert (isptr (space_start (heap_head (ti_heap t_info')))) by 
+   (eapply space_start_isptr'; eassumption).
+ sep_apply get_tinfo_alloc.
+ Intros.
+ set (JJ :=  _ -* _).
+ limited_change_compspecs CompSpecs.
+ forward.
+ subst JJ.
+ set (KK := field_at _ _ _ _ _).
+ sep_apply (modus_ponens_wand KK).
+ clear KK.
+ change (Tpointer _ _) with int_or_ptr_type.
+ set (new0 := offset_val _ _).
+ rewrite (split2_data_at__Tarray_app 1) by lia.
+ Intros.
+ forward.
+ change (default_val (tarray int_or_ptr_type 1)) with [Vundef].
+ rewrite upd_Znth0 by lia.
+ set (new1 := field_address0 (tarray int_or_ptr_type n) (SUB 1) new0).
+ sep_apply data_at__memory_block_cancel.
+ assert (0 <= 8 * (n - 1) < Ptrofs.modulus). {
+  Search total_space.
+   pose proof (total_space_tight_range (heap_head (ti_heap t_info'))).
+   pose proof (space_order (heap_head (ti_heap t_info'))).
+   clear - H7 H9 H10 H99. unfold MAX_SPACE_SIZE in H9. simpl in H9.
+   really_simplify Ptrofs.modulus.
+   set (tot := total_space _) in *. set (use := used_space _) in *.
+   clearbody tot. clearbody use. clearbody n. clear - H7 H9 H10 H99.
+   split; try lia.
+ }
+ sep_apply memory_block_data_at__tarray_tuchar.
+ simpl. rewrite Z.max_r by lia. auto. 
+ simpl sizeof. rewrite Z.max_r by lia.
+ replace (8 * (n-1)) with (len + pad_length).
+2:{
+ subst n.
+ rewrite <- Z.add_sub_assoc.
+ change (1-1) with 0.
+ rewrite Z.add_0_r.
+ rewrite <- Z_div_exact_2; try lia.
+ subst pad_length.
+ rewrite Z.add_sub_assoc.
+ rewrite Z.add_comm.
+ rewrite <- Z.add_sub_assoc.
+ rewrite Zplus_mod.
+ simpl.
+ rewrite Zminus_mod.
+ rewrite !Zmod_mod.
+ rewrite Z.sub_diag. reflexivity.
+ }
+ 
+
 (* Still some work to do *)
  
 Abort.
